% !TEX TS-program = lualatex
\documentclass[notoc,notitlepage]{tufte-book}
% \nonstopmode % uncomment to enable nonstopmode

\usepackage{classnotetitle}

\title{PMATH348 --- Fields and Galois Theory}
\author{Johnson Ng}
\subtitle{Classnotes for Winter 2019}
\credentials{BMath (Hons), Pure Mathematics major, Actuarial Science Minor}
\institution{University of Waterloo}

\input{latex-classnotes-preamble.tex}

\DeclareMathOperator{\stab}{Stab}
\DeclareMathOperator{\orb}{Orb}

\begin{document}
\input{latex-classnotes-header.tex}

\chapter*{Preface}%
\addcontentsline{toc}{chapter}{Preface}
\label{chp:preface}
% chapter preface

This is a 3 part course; it is separated into
\begin{enumerate}
  \item \textbf{Sylow's Theorem}

    which is a leftover from group theory (\href{https://tex.japorized.ink/PMATH347S18/classnotes.pdf}{PMATH 347}). It has little to do with the rest of the course, but PMATH 347 was a course that is already content-rich to a point where Sylow's Theorem gets pushed into the later course that is this course.

  \item \textbf{Field Theory}

    is a somewhat understood concept from ring theory, where we learned that it is a special case of a ring where all of its elements have an inverse.

  \item \textbf{Galois Theory}

    is the beautiful theory from the French mathematican Ã‰variste Galois that ties field theory back to group theory. This allows us to reduce certain field theory problems into group theory, which, in some sense, is easier and better understood.
\end{enumerate}

% chapter preface (end)

\part{Sylow's Theorem}

\chapter{Lecture 1 Jan 07th}%
\label{chp:lecture_1_jan_07th}
% chapter lecture_1_jan_07th

\section{Cauchy's Theorem}%
\label{sec:cauchy_s_theorem}
% section cauchy_s_theorem

Recall Lagrange's Theorem.

\begin{thm}[Lagrange's Theorem]\index{Lagrange's Theorem}\label{thm:lagrange_s_theorem}
  If $G$ is a finite group and $H$ is a subgroup of $G$ \sidenote{I shall write this as $H \leq G$ from hereon.}, then $\abs{H} \mid \abs{G}$ \sidenote{This just means $\abs{H}$ divides $\abs{G}$.}.
\end{thm}

The full converse is not true.

\begin{eg}
  Let $G = A_4$, the \hlnotea{alternating group} of $4$ elements. Then $\abs{G} = 12$ \sidenote{Recall that the symmetric group of $4$ elements $S_4$ has order $4! = 24$, and an alternating group has half of its elements.}. We have that $6 \mid 12$. We shall show that $G$ has no subgroup of order $6$.

  Suppose to the contrary that $H \leq G$ such that $\abs{H} = 6$. Let $a \in G$ such that $\abs{a} = 3$ \sidenote{i.e. the order of $a$ is $3$. This is a \hlimpo{trick}.} There are $8$ such elements in $G$ \sidenote{This shall be left as an exercise.
  \begin{ex}
    Prove that there are $8$ elements in $G$ that have order $3$.
  \end{ex}}. Note that the \hlnotea{index}\sidenote{The index of a subgroup is the number of unique cosets generated by $H$.} of $H$, $\abs{G : H}$, is $\frac{\abs{G}}{\abs{H}} = 2$.

  Now consider the \hlnotea{cosets} $H$, $aH$ and $a^2 H$. Since $\abs{G : H} = 2$, we must have either
  \begin{itemize}
    \item $aH = H \implies a \in H$;
    \item $aH = a^H \overset{\text{`multiply' } a^{-1}}{\implies} H = aH \implies a \in H$; or
    \item $a^2H = H \overset{\text{`multiply' } a}{\implies} H = aH \implies a \in H$.
  \end{itemize}
  Thus all $8$ elements of order $3$ are in $H$ but $\abs{H} = 6$, a contradiction. Therefore, no such subgroup (of order $6$) exists.
\end{eg}

Our goal now is to establish a partial converse of Lagrange's Theorem. To that end, we shall first lay down some definitions.

\begin{defn}[$p$-Group]\index{$p$-Group}\label{defn:_p_group}
  Let $p$ be prime. We say that a group $G$ is a \hlnoteb{$p$-group} if $\abs{G} = p^k$ for some $k \in \mathbb{N}$. For $H \leq G$, we say that $H$ is a $p$-subgroup of $G$ if $H$ is a $p$-group.
\end{defn}

\begin{defn}[Sylow $p$-Subgroup]\index{Sylow $p$-Subgroup}\label{defn:sylow_p_subgroup}
  Let $G$ be a group such that $\abs{G} = p^n m$ for some $n, m \in \mathbb{N}$, such that $p \nmid m$. If $H \leq G$ with order $p^n$, we call $H$ a \hlnoteb{Sylow $p$-subgroup}.
\end{defn}

Recall Cauchy's Theorem for abelian groups\sidenote{In the course I was in, we were introduced only to the full theorem and actually went through this entire part. See notes on \href{https://tex.japorized.ink/PMATH347S18/classnotes.pdf}{PMATH 347}.}.

\begin{thm}[Cauchy's Theorem for Abelian Groups]\index{Cauchy's Theorem for Abelian Groups}\label{thm:cauchy_s_theorem_for_abelian_groups}
  If $G$ is a finite abelian group, and $p$ is prime such that $p \mid \abs{G}$, then $\abs{G}$ has an element of order $p$.
\end{thm}

\begin{defn}[Stabilizers and Orbits]\index{Stabilizers}\index{Orbits}\label{defn:stabilizers_and_orbits}
  Let $G$ be a finite group which acts on a finite set $X$ \sidenote{Recall that a group action is a function $\cdot : G \times X \to X$ such that
  \begin{enumerate}
    \item $g(hx) = (gh)x$; and
    \item $ex = x$.
  \end{enumerate}}. For $x \in X$, the \hlnoteb{stabilizers} of $x$ is the set
  \begin{equation*}
    \stab(x) := \{ g \in G : g x = x \} \leq G.
  \end{equation*}
  The orbits of $x$ is a set
  \begin{equation*}
    \orb(x) := \{ gx : g \in G \}.
  \end{equation*}
\end{defn}

\begin{note}
  One can verify that the function $G / \stab(x) \to \orb(x)$ such that
  \begin{equation*}
    g \stab(x) \mapsto gx
  \end{equation*}
  is a bijection.
\end{note}

\begin{thm}[Orbit-Stabilizer Theorem]\index{Orbit-Stabilizer Theorem}\label{thm:orbit_stabilizer_theorem}
  Let $G$ be a group acting on a set $X$, and for each $x \in X$, $\stab(x)$ and $\orb(x)$ are the stabilizers and orbits of $x$, respectively. Then
  \begin{equation*}
    \abs{G} = \abs{\stab(x)} \cdot \abs{\orb(x)}.
  \end{equation*}
  Moreover, if $x, y \in X$, then either $\orb(x) \cap \orb(y) = \emptyset$ or $\orb(x) = \orb(y)$.
\end{thm}

The theorem is actually equivalent to \href{https://tex.japorized.ink/PMATH347S18/classnotes.pdf#thm.45}{Proposition 45} in the notes for PMATH 347. However, feel free to...

\begin{ex}
  prove \cref{thm:orbit_stabilizer_theorem} as an exercise.
\end{ex}

Consequently, we have that
\begin{equation*}
  \abs{X} = \sum \abs{\orb(a_i)},
\end{equation*}
where $a_i$ are the distinct orbit representatives. Letting
\begin{equation*}
  X_G := \{ x \in X : gx = x, g \in G \},
\end{equation*}
we have...

\begin{thm}[Orbit Decomposition Theorem]\index{Orbit Decomposition Theorem}\label{thm:orbit_decomposition_theorem}
  \begin{equation*}
    \abs{X} = \abs{X_G} + \sum_{a_i \notin X_G} \abs{\orb(a_i)}.
  \end{equation*}
\end{thm}

% section cauchy_s_theorem (end)

% chapter lecture_1_jan_07th (end)

\chapter{Lecture 2 Jan 09th}%
\label{chp:lecture_2_jan_09th}
% chapter lecture_2_jan_09th

\section{The Sylow Theorems}%
\label{sec:the_sylow_theorems}
% section the_sylow_theorems

From the \hyperref[thm:orbit_decomposition_theorem]{Orbit Decomposition Theorem}, one special case is when $G$ acts on $X = G$ by conjugation.

\begin{crly}[Class Equation]\index{Class Equation}\label{crly:class_equation}
  From \cref{thm:orbit_decomposition_theorem}, if $X = G$, we have
  \begin{align*}
    \abs{G} &= \abs{Z(G)} + \sum \overarrow{\abs{ \orb(a_i) }}{\text{non-central}} \\
            &= \abs{Z(G)} + \sum [ G : \stab(a_i) ] \text{ by } \hyperref[thm:orbit_stabilizer_theorem]{Orbit-Stabilizer} \\
            &= \abs{Z(G)} + \sum [ G : C(a_i) ],
  \end{align*}
  where $C(a_i)$ is called the \hldefn{centralizers} of $G$. 
\end{crly}

\begin{thm}[First Sylow Theorem]\index{First Sylow Theorem}\label{thm:first_sylow_theorem}
  Let $G$ be a finite group, and let $p \mid \abs{G}$ such that $p$ is prime.
  Then $G$ contains a Sylow $p$-subgroup.
\end{thm}

\begin{proof}
  We proceed by induction on the size of $G$.
  If $\abs{G} = 2$, then $p = 2$, and so $G$ is its own Sylow $p$-subgroup
  \sidenote{A $2$-cycle is a Sylow $p$-group.}.
  
  Consider a finite group $G$ with $\abs{G} \geq 2$.
  Let $p$ be a prime that divides $\abs{G}$, and assume
  that the desired result holds for smaller groups.
  
  Let $\abs{G} = p^n m$, where $n, m \in \mathbb{N}$, and $p \nmid m$.

  \noindent
  \hlbnotea{Case 1: $p \mid \abs{Z(G)}$}
  By \cref{thm:cauchy_s_theorem_for_abelian_groups}, $\exists a \in Z(G)$
  such that $\abs{a} = p$.
  Since $\langle a \rangle \subsetneq Z(G)$, we have that
  \begin{equation*}
    \langle a \rangle \triangleleft G \text{ and } \abs{ \langle a \rangle } = p.
  \end{equation*}
  \sidenote{This feels like a struck of genius.
  Let's break it down and find some way that makes it easier to remember.
  We want to find $H \leq G$ such that $\abs{H} = p^n$.
  We have $\abs{ \langle a \rangle } = p$.
  We want to be able to use the \hlimpo{Correspondence Theorem},
  so we should adjust our materials to fit that mold:
  since $\abs{\langle a \rangle} = p$, notice that
  \begin{equation*}
    \frac{\abs{G}}{\abs{\langle a \rangle}} = p^{n - 1} m.
  \end{equation*}
  This is a smaller group than $G$, and so IH tells us that it
  has a Sylow $p$-subgroup, say $\bar{H}$.
  By the Correspondence Theorem, we may retrieve $H$.}
  Notice that the group $G / \langle a \rangle$ is a group
  that has a lower order than $G$, and so by IH,
  $\exists \bar{H} \leq G / \langle a \rangle$ such that $\bar{H}$
  is a Sylow $p$-subgroup of $G / \langle a \rangle$.
  Note that if $n = 1$. then $\langle a \rangle$ itself is the
  Sylow $p$-subgroup.
  WMA $n > 1$. We have that $\abs{H} = p^{n - 1}$.
  By \hyperref[thm:correspondence_theorem]{correspondence},
  \begin{equation*}
    \bar{H} = H / \langle a \rangle,
  \end{equation*}
  where $H \leq G$. By comparing the orders, we have
  \begin{equation*}
    p^{n - 1} = \frac{\abs{H}}{p} \implies \abs{H} = p^n.
  \end{equation*}
  Therefore $H$ is a Sylow $p$-subgroup of $G$.

  \noindent
  \hlbnotea{Case 2: $p \nmid Z(G)$}
  By the \hyperref[crly:class_equation]{class equation},
  notice that
  \begin{equation}\label{eq:first_sylow_theorem_eq1}
    p^n m = \abs{G} = \abs{Z(G)} + \sum [ G : C(a_i) ],
  \end{equation}
  and the summation cannot be $0$ or $p$ would otherwise
  divide $Z(G)$.
  \marginnote{This highlighted part requires clarification.}
  % TODO: this needs the prof's intervention
  \begin{quotebox}{be-red}{light}
  Since $p$ divides the LHS of \cref{eq:first_sylow_theorem_eq1}
  and not $\abs{Z(G)}$, and the sum is nonzero, we must 
  have that $\exists a_i \in G$ such that $p \nmid [ G : C(a_i) ]$.
  This implies that $p^n \mid \abs{ C(a_i) }$.
  \end{quotebox}
  Since $a_i \notin Z(G)$, we have $\abs{C(a_i)} \leq \abs{G}$.
  Thus by IH, $C(a_i)$ has a Sylow $p$-subgroup, which is also a
  Sylow $p$-subgroup of $G$.\qed\
\end{proof}

\begin{crly}[Cauchy's Theorem]\index{Cauchy's Theorem}\label{crly:cauchy_s_theorem}
  If $p$ is prime and $p \mid \abs{G}$, then $G$ has an element of order $p$.
\end{crly}

\begin{proof}
  WLOG, WMA $\abs{G} = p^n m$, where $n, m \in \mathbb{N}$ and
  $p \nmid m$. By \cref{thm:first_sylow_theorem}, $\exists H \leq G$
  such that $H$ is a Sylow $p$-subgroup.
  Take $a \in H \setminus \left\{ e \right\}$. Then $\abs{a} = p^k$
  for some $k \leq n$.

  Let $b = a^{p^{k - 1}}$. Notice that $b \neq e$, or it would
  contradict the definition of an order (for $a$).
  Then $b^p = \left( a^{p^{k - 1}} \right)^p = a^p = e$.
  Therefore $\abs{b} = p$ and $b \in G$.\qed\
\end{proof}

\begin{defn}[Normalizer]\index{Normalizer}\label{defn:normalizer}
  Let $G$ be a group, and $H \leq G$. The set
  \begin{equation*}
    N_G(H) = \left\{ g \in G \mmid gHg^{-1} = H \right\}
  \end{equation*}
  is called the \hlnoteb{normalizer} of $H$ in $G$.
\end{defn}

\begin{ex}
  Verify that $N_G(H)$ is the largest subgroup of $G$
  that contains $H$ as a normal subgroup.
\end{ex}

\begin{proof}
  It is clear by definition of a normalizer that $H \triangleleft N_G(H)$.

  Suppose there exists $N_G(H) < \tilde{H} \leq G$ such that
  $H \triangleleft \tilde{H}$. Let $h \in \tilde{H} \setminus N_G(H)$.
  But since $H \triangleleft \tilde{H}$, we have
  \begin{equation*}
    hHh^{-1} = H,
  \end{equation*}
  which implies that $h \in N_G(H)$, a contradiction.
  Therefore $N_G(H)$ is the largest subgroup that contains $H$ as a
  normal subgroup.
\end{proof}

Before proceeding with the Sylow's next theorem, we require two lemmas.

\begin{lemma}[Intersection of a Sylow $p$-subgroup with any other $p$-subgroups]\label{lemma:intersection_of_a_sylow_p_subgroup_with_any_other_p_subgroups}
  Let $G$ be a finite group and $p$ a prime such that $p \mid \abs{G}$.
  Let $P, Q \leq G$ be a Sylow $p$-subgroup and a (regular) $p$-subgroup,
  respectively. Then
  \begin{equation}\label{eq:intersection_of_a_sylow_p_subgroup_with_any_other_p_subgroups}
    Q \cap N_G(P) = Q \cap P.
  \end{equation}
\end{lemma}

\begin{proof}
  Since $P \subseteq N_G(P)$, $\subseteq$ of \cref{eq:intersection_of_a_sylow_p_subgroup_with_any_other_p_subgroups} is done.

  Let $N = N_G(P)$, and let $H = Q \cap N$. WTS $H \subseteq Q \cap P$.
  Since $H = Q \cap N \subseteq Q$, it suffices to show that $H \subseteq P$.
  Since $P$ is a Sylow $p$-subgroup, let $\abs{P} = p^n$. By Lagrange,
  we have that $\abs{H} = p^m$ for some $m \leq n$. Since $P \trianglleft N$,
  we have that $HP \leq N$ 
  \sidenote{See \href{https://tex.japorized.ink/PMATH347S18/classnotes.pdf\#thm.30}{PMATH 347}}.
  Moreover, we have that
  \begin{equation*}
    \abs{HP} = \frac{\abs{H}\abs{P}}{\abs{H \cap P}} = p^k
  \end{equation*}
  for some $k \leq n$. Also, $P \subset HP$, and so $n \leq k$,
  implying that $k = n$. Thus $P = HP$, and thus
  \begin{equation*}
    H \subseteq HP = P,
  \end{equation*}
  as required.\qed\
\end{proof}

% section the_sylow_theorems (end)

% chapter lecture_2_jan_09th (end)

\chapter{Lecture 3 Jan 11th}%
\label{chp:lecture_3_jan_11th}
% chapter lecture_3_jan_11th

\section{The Sylow Theorems (Continued)}%
\label{sec:the_sylow_theorems_continued}
% section the_sylow_theorems_continued

\begin{lemma}[Counting The Conjugates of a Sylow $p$-Subgroup]\label{lemma:counting_the_conjugates_of_a_sylow_p_subgroup}
  Let $G$ be a finite group, and $p$ a prime such that $p \mid \abs{G}$. Let
  \begin{itemize}
    \item $P$ be a Sylow $p$-subgroup;
    \item $Q$ be a $p$-subgroup;
    \item $K = \left\{ gPg^{-1} \mmid g \in G \right\}$;
    \item $Q$ act on $K$ by conjugation; and
    \item $P = P_1, P_2, \ldots, P_r$ be the distinct orbit representatives
      from the action of $Q$ on $K$.
  \end{itemize}
  Then
  \begin{equation*}
    \abs{K} = \sum_{i=1}^{r} \left[ Q : Q \cap P_i \right].
  \end{equation*}
\end{lemma}

\begin{proof}
  From the definition of $K$, and the fact that $Q$ acts on $K$,
  we have
  \begin{align*}
    \abs{K} &= \sum_{i=1}^{r} \abs{ \Orb(P_i) } \\
            &= \sum_{i=1}^{r} \abs{ Q } / \abs{ \stab(P_i) } \quad \hyperref[thm:orbit_stabilizer_theorem]{\text{orbit-stabilizer}} \\
            &= \sum_{i=1}^{r} \abs{ Q } / \abs{ N_G(P_i) \cap Q } \quad \text{ by the action } \\
            &= \sum_{i=1}^{r} [ Q : N_G(P_i) \cap Q ] \quad \text{ by definition } \\
            &= \sum_{i=1}^{r} [ Q : Q \cap P_i ] \quad \hyperref[lemma:intersection_of_a_sylow_p_subgroup_with_any_other_p_subgroups]{\text{the last lemma}}.
  \end{align*}\qed\
\end{proof}

\begin{thm}[Second Sylow Theorem]\index{Second Sylow Theorem}\label{thm:second_sylow_theorem}
  If $P$ and $Q$ are Sylow $p$-subgroups of $G$, then
  $\exists g \in G$ such that $P = gQg^{-1}$.
\end{thm}

\begin{proof}
  Let $K = \left\{ qPq^{-1} \mmid q \in G \right\}$. WTS $Q \in K$.
  We shall also note that $\abs{P} = p^k$ for some $k \in \mathbb{N}$.

  Let $P$ act on $K$ by conjugation. Let the orbit representatives be
  \begin{equation*}
    P = P_1, P_2, \ldots, P_r.
  \end{equation*}
  By \cref{lemma:counting_the_conjugates_of_a_sylow_p_subgroup}, we have
  \begin{equation*}
    \abs{K} = \sum_{i=1}^{r} [ P : P \cap P_i ] 
            = [ P : P ] + \sum_{i=2}^{r} [ P : P \cap P_i ]
            = 1 + \sum_{i=2}^{r} [ P : P \cap P_i ].
  \end{equation*}
  Thus
  \begin{equation*}
    \abs{K} \equiv 1 \mod p.
  \end{equation*}

  Now let $Q$ act on $K$ by conjugation. Reordering if necessary, the
  orbit representatives are
  \begin{equation*}
    P = P_1, P_2, \ldots, P_s,
  \end{equation*}
  where $s$ is not necessarily $r$. From here, it suffices to show that
  $Q = P_i$ for some $i \in \left\{ 1, 2, \ldots, s \right\}$. Suppose
  not. Then by \cref{lemma:counting_the_conjugates_of_a_sylow_p_subgroup},
  \begin{equation*}
    \abs{K} = \sum_{i=1}^{s} [ Q : P_i \cap Q ].
  \end{equation*}
  Note that it must be the case that $[ Q : P_i \cap Q ] > 1$, for some if
  not all $i$, for otherwise it would imply that $Q \cap P_i$ and that would
  be a contradiction. Then by Lagrange,
  \begin{equation*}
    \abs{K} \equiv 0 \mod p.
  \end{equation*}
  This contradicts the fact that $\abs{K} \equiv 1 \mod p$.

  This shows that $Q = P_i$ for some $i \in \left\{ 1, 2, \ldots, s \right\}$,
  and so $Q$ is a conjugate of $P$.\qed\
\end{proof}

\begin{note}[Notation]
  We shall denote $n_p$ as the number of Sylow $p$-subgroups in $G$.
\end{note}

\begin{thm}[Third Sylow Theorem]\index{Third Sylow Theorem}\label{thm:third_sylow_theorem}
  Let $p$ be a prime, and that it divides $\abs{G}$, where $G$ is a group.
  Suppose $\abs{G} = p^n m$, where $n, m \in \mathbb{N}$ and $p \nmid m$.
  Then
  \begin{enumerate}
    \item $n_p \equiv 1 \mod p$; and
    \item $n_p \mid m$.
  \end{enumerate}
\end{thm}

\begin{proof}
  Let $P$ be a Sylow $p$-subgroup of $G$, and let
  \begin{equation*}
    K = \left\{ gPg^{-1} \mmid g \in G \right\}.
  \end{equation*}
  By \hyperref[thm:second_sylow_theorem]{Sylow's second theorem},
  $n_p = \abs{K}$ as all the conjugates are exactly the Sylow
  $p$-subgroups. And by our last proof, we saw that $n_p \equiv 1 \mod p$.

  Let $G$ act on $K$ by conjugation. Then by the \hyperref[thm:orbit_stabilizer_theorem]{Orbit-Stabilizer Theorem},
  \begin{equation*}
    \abs{G} = \abs{\stab(P)}\abs{\orb(P)}.
  \end{equation*}
  Thus
  \begin{equation}\label{eq:third_sylow_theorem_eq1}
    p^n m = \abs{ N_G(P) } n_p.
  \end{equation}
  Thus $n_p \mid p^n m$. Since $n_p \equiv 1 \not\equiv 0 \mod p$,
  we must have $n_p \mid m$.\qed\
\end{proof}

\begin{remark}
  \begin{enumerate}
    \item From \cref{eq:third_sylow_theorem_eq1}, we have that
      \begin{equation*}
        n_p = [ G : N_G(P) ].
      \end{equation*}
    \item \imponote\ Note that
      \begin{equation*}
        n_p \equiv 1 \mod p \iff \forall g \in G gPg^{-1} = P \iff P \triangleleft G.
      \end{equation*}
  \end{enumerate}
\end{remark}

\begin{defn}[Simple Group]\index{Simple Group}\label{defn:simple_group}
  A group is said to be \hlnoteb{simple} if it has no non-trivial normal subgroups.
\end{defn}

\begin{eg}
  Prove that there is no simple group of order $56$.
\end{eg}

\begin{proof}
  Let $G$ be a group.
  Note that $56 = 2^3 \cdot 7$. Then $n_7 \equiv 1 \mod 7$ and
  $n_7 \mid 8 = 2^3$. Thus
  \begin{equation*}
    n_7 = 1 \text{ or } n_7 = 8.
  \end{equation*}

  \hlbnotea{$n_7 = 1$} By the remark above, $G$ has a normal Sylow
  $7$-subgroup. Thus $G$ is not simple.

  \hlbnotea{$n_7 = 8$} By Lagrange, since $7$ is prime, the distinct
  Sylow $7$-subgroups of $G$ intersect trivially. Therefore, there
  are $8 \times 6 = 48$ elements of order $7$ in $G$. But this
  implies that $56 - 48 = 8$ elements that are not of order $7$.
  One of them is the identity, thus the remaining $7$ elements must have
  order $2$ \sidenote{They cannot be of any other order as that would
  create a cyclic group that is not of order $2$ or $7$, which is
  impossible.}. This implies that
  \begin{equation*}
    n_2 = 7 \equiv 1 \mod 2,
  \end{equation*}
  which by our remark means that $G$ has a normal Sylow $2$-subgroup.
  Thus $G$ is not simple by both accounts.
\end{proof}

% section the_sylow_theorems_continued (end)

% chapter lecture_3_jan_11th (end)

\appendix

\chapter{Asides and Prior Knowledge}%
\label{chp:asides_and_prior_knowledge}
% chapter asides_and_prior_knowledge

\section{Correspondence Theorem}%
\label{sec:correspondence_theorem}
% section correspondence_theorem

\hlnotea{The Correspondence Theorem} is somewhat widely known 
as the Fourth Isomorphism Theorem, although some authors associates
the name with a proposition known as 
\href{https://en.wikipedia.org/wiki/Zassenhaus_lemma}{Zaessenhaus Lemma}.

\begin{thm}[Correspondence Theorem]\index{Correspondence Theorem}\label{thm:correspondence_theorem}
  Let $G$ be a group, and $N \triangleleft G$
  \sidenote{Recall that this symbol means that $N$ is a normal
  subgroup of $G$.}. Then there exists a bijection between
  the set of all subgroups $A \leq G$ such that $A \supseteq N$
  and the set of subgroups $A / N$ of $G / N$.
\end{thm}

\begin{proof}
  % TODO: prove the Correspondence Theorem
\end{proof}

% section correspondence_theorem (end)

% chapter asides_and_prior_knowledge (end)

\backmatter

\pagestyle{plain}

\nobibliography*
\bibliography{references}

\printindex

\end{document}

